src/Dafny/typeConversions.i.dfy
@@ -6,64 +6,108 @@ module type_conversion {
 
 
 
-    function evalSEXT(t0:Value,src:Value,t1:Value): Value
+    function evalZEXT(t0:Value,src:Value,t1:Value): Value
         requires typesMatch(t0,src)
+        requires unsignedVal(src)
+        requires unsignedVal(t1)
+        requires unsignedValLT(src,t1)
     {
-        
-        if t1.Val8? then evalSEXT8Helper(src) else 
-        if t1.Val16? then evalSEXT16Helper(src) else 
-        if t1.Val32? then evalSEXT32Helper(src) else 
-        if t1.Val64? then evalSEXT64Helper(src) else 
-        if t1.Val128? then evalSEXT128Helper(src) else 
+        if t1.Val8? then evalZEXT8Helper(src) else 
+        if t1.Val16? then evalZEXT16Helper(src) else 
+        if t1.Val32? then evalZEXT32Helper(src) else 
+        if t1.Val64? then evalZEXT64Helper(src) else 
+        if t1.Val128? then evalZEXT128Helper(src) else 
         src
     }
 
-    function evalSEXT8Helper(src:Value) : Value
+    function evalZEXT8Helper(src:Value) : Value
     {
-        if src.Val8? then src else 
-        if src.Val16? then Val8(Bitwise16CastTo8(src.v16)) else
-        if src.Val32? then Val8(Bitwise32CastTo8(src.v32)) else
-        if src.Val64? then Val8(Bitwise64CastTo8(src.v64)) else
-        if src.Val64? then Val8(Bitwise128CastTo8(src.v128)) else 
-                            src
+       src
     }
 
-    function evalSEXT16Helper(src:Value) : Value
+    function evalZEXT16Helper(src:Value) : Value
     {
-        if src.Val8? then Val16(Bitwise8CastTo16(src.v8)) else 
-        if src.Val16? then src else
-        if src.Val32? then Val16(Bitwise32CastTo16(src.v32)) else
-        if src.Val64? then Val16(Bitwise64CastTo16(src.v64)) else
-        if src.Val64? then Val16(Bitwise128CastTo16(src.v128)) else 
-                            src
+        if src.Val8? then Val16(Bitwise8CastTo16(src.v8)) else src
     }
 
-    function evalSEXT32Helper(src:Value) : Value
+    function evalZEXT32Helper(src:Value) : Value
     {
         if src.Val8? then Val32(Bitwise8CastTo32(src.v8)) else 
-        if src.Val16? then Val32(Bitwise16CastTo32(src.v16)) else
-        if src.Val32? then src else
-        if src.Val64? then Val32(Bitwise64CastTo32(src.v64)) else
-        if src.Val64? then Val32(Bitwise128CastTo32(src.v128)) else 
-                            src
+        if src.Val16? then Val32(Bitwise16CastTo32(src.v16)) else src 
     }
 
-    function evalSEXT64Helper(src:Value) : Value
+    function evalZEXT64Helper(src:Value) : Value
     {
         if src.Val8? then Val64(Bitwise8CastTo64(src.v8)) else 
         if src.Val16? then Val64(Bitwise16CastTo64(src.v16)) else
-        if src.Val32? then Val64(Bitwise32CastTo64(src.v32)) else
-        if src.Val64? then src else
-        if src.Val128? then Val64(Bitwise128CastTo64(src.v128)) else 
-                            src
+        if src.Val32? then Val64(Bitwise32CastTo64(src.v32)) else src
     }
 
-    function evalSEXT128Helper(src:Value) : Value
+    function evalZEXT128Helper(src:Value) : Value
     {
         if src.Val8? then Val128(Bitwise8CastTo128(src.v8)) else 
         if src.Val16? then Val128(Bitwise16CastTo128(src.v16)) else
         if src.Val32? then Val128(Bitwise32CastTo128(src.v32)) else
-        if src.Val64? then Val128(Bitwise64CastTo128(src.v64)) else 
-                            src
+        if src.Val64? then Val128(Bitwise64CastTo128(src.v64)) else src
     }
+
+
+///// Cast functions /////
+
+////----UNSIGNED----////
+
+//
+function {:opaque} Bitwise8CastTo16(x:uint8):uint16
+{
+    x  % 0x1000
+}
+//
+function {:opaque} Bitwise8CastTo32(x:uint8):uint32
+{
+    x  % 0x1_0000_0000
+}
+function {:opaque} Bitwise16CastTo32(x:uint16):uint32
+{
+    x  % 0x1_0000_0000
+}
+//
+function {:opaque} Bitwise8CastTo64(x:uint8):uint64
+{
+    x  % 0x1_0000_0000_0000_0000
+}
+function {:opaque} Bitwise16CastTo64(x:uint16):uint64
+{
+    x  % 0x1_0000_0000_0000_0000
+}
+function {:opaque} Bitwise32CastTo64(x:uint32):uint64
+{
+    x  % 0x1_0000_0000_0000_0000
+}
+//
+function {:opaque} Bitwise8CastTo128(x:uint8):uint128
+{
+    x  % 0x1_00000000_00000000_00000000_00000000
+}
+function {:opaque} Bitwise16CastTo128(x:uint16):uint128
+{
+    x  % 0x1_00000000_00000000_00000000_00000000
+}
+function {:opaque} Bitwise32CastTo128(x:uint32):uint128
+{
+    x  % 0x1_00000000_00000000_00000000_00000000
+}
+function {:opaque} Bitwise64CastTo128(x:uint64):uint128
+{
+    x  % 0x1_00000000_00000000_00000000_00000000
+}
+
+////----SIGNED----////
+
+function {:opaque} SignedBitwise8CastTo16(x:sint8):sint16
+{
+    x  % 0x8000
+}
+
+
+
 }
